ironfleet/src/Dafny/Distributed/Protocol/Pb/PerformanceProof/Proof.i.dfy
@@ -1,0 +1,294 @@
+include "TimestampedSystem.i.dfy"
+include "TimeBounds.i.dfy"
+
+module Performance_Proof {
+import opened TimestampedPbSystem_i
+import opened TimeBounds_i
+
+predicate Consistency(ps:TimestampedPbState)
+{
+  |ps.t_nodes| == |ps.constants.config|
+    && |ps.t_nodes| > 0
+    && (forall i :: 0 <= i < |ps.t_nodes| ==> ps.t_nodes[i].v.con == ps.constants)
+    && (forall i :: 0 <= i < |ps.t_nodes| ==> ps.t_nodes[i].v.myIndex == i)
+}
+
+type InvType = (TimestampedPbState --> bool)
+
+predicate isInv(inv:InvType)
+{
+  && (forall ps :: Consistency(ps) ==> inv.requires(ps))
+  && (forall ps, con :: TimestampedPbInit(con, ps) ==> Consistency(ps) ==> inv(ps))
+  && (forall ps, ps' :: TimestampedPbNext(ps, ps') ==>
+      Consistency(ps) ==> inv(ps) ==> Consistency(ps') ==> inv(ps'))
+}
+
+predicate invImpliesInv(A:InvType, B:InvType)
+{
+  && (forall ps :: Consistency(ps) ==> A.requires(ps))
+  && (forall ps :: Consistency(ps) ==> B.requires(ps))
+
+  && (forall ps, con :: TimestampedPbInit(con, ps) ==> Consistency(ps) ==> A(ps) ==> B(ps))
+  && (forall ps, ps' :: TimestampedPbNext(ps, ps') ==>
+      Consistency(ps) ==> Consistency(ps') ==>
+      B(ps) ==> A(ps) ==> A(ps') ==> B(ps'))
+}
+
+function andInv(A:InvType, B:InvType) : InvType
+{
+  (ps:TimestampedPbState) requires (A.requires(ps) && B.requires(ps)) =>
+    (A(ps) && B(ps))
+}
+
+////////////////////////////////////////////////////////////////////////////////
+
+predicate Inv_Primary(ps:TimestampedPbState)
+  requires Consistency(ps)
+{
+  ps.t_nodes[0].v.nextStep == 0 ==>
+    ps.t_nodes[0].ts == TimeZero()
+}
+
+lemma lemma_Inv_Primary()
+  ensures isInv(Inv_Primary)
+{
+  forall ps, con |
+    TimestampedPbInit(con, ps) && Consistency(ps)
+    ensures Inv_Primary(ps)
+  {}
+
+  forall ps, ps' |
+    TimestampedPbNext(ps, ps') && Consistency(ps) && Consistency(ps') && Inv_Primary(ps)
+    ensures Inv_Primary(ps')
+  {}
+}
+
+////////////////////////////////////////////////////////////////////////////////
+
+predicate requestPacketInv(con:Constants, pkt:TimestampedPbPacket)
+  requires |con.config| > 0
+  requires pkt.msg.v.Request?
+{
+    TimeEq(pkt.msg.ts, RequestPacketT())
+      && pkt.src == con.config[0]
+}
+
+predicate Inv_RequestPacket(ps:TimestampedPbState)
+  requires Consistency(ps)
+{
+  forall pkt :: pkt in ps.t_environment.sentPackets ==> pkt.msg.v.Request? ==>
+    requestPacketInv(ps.constants, pkt)
+}
+
+lemma lemma_Inv_RequestPacket()
+  ensures invImpliesInv(Inv_Primary, Inv_RequestPacket)
+{
+  forall ps, con |
+    TimestampedPbInit(con, ps) && Consistency(ps)
+    && Inv_Primary(ps)
+    ensures Inv_RequestPacket(ps)
+  {}
+
+  forall ps, ps' |
+    TimestampedPbNext(ps, ps') && Consistency(ps) && Consistency(ps') && Inv_RequestPacket(ps)
+    && Inv_Primary(ps) && Inv_Primary(ps')
+    ensures Inv_RequestPacket(ps')
+  {
+    /*
+    forall pkt |
+      pkt in ps'.t_environment.sentPackets && pkt.msg.v.Request?
+      ensures requestPacketInv(ps.constants, pkt)
+    {
+      if pkt in ps.t_environment.sentPackets {
+        assert requestPacketInv(ps.constants, pkt);
+      } else {
+        var ios := ps.t_environment.nextStep.ios;
+
+        assert !ios[0].LIoOpReceive?;
+        assert !ios[0].LIoOpTimeoutReceive?;
+
+        assert pkt in (set io | io in ios && io.LIoOpSend? :: io.s);
+        var io :| io in ios && io.LIoOpSend? && io.s == pkt;
+        assert pkt.msg.ts == ps'.t_nodes[0].ts + D;
+        assert ps'.t_nodes[0].ts == TimeZero() + PrimaryReqT;
+
+        assert pkt.src == ps'.constants.config[0];
+
+        // assert pkt.ts == ps'.t_nodes[idx].ts + D;
+        assert requestPacketInv(ps.constants, pkt);
+      }
+    }
+    */
+  }
+}
+
+////////////////////////////////////////////////////////////////////////////////
+
+// Bounded queueing assumption
+predicate QAssumption(s:TimestampedPbState)
+  requires Consistency(s)
+{
+  forall idx, ios, hstep :: 0 <= idx < |s.constants.config|
+    ==> s.t_environment.nextStep == LEnvStepHostIos(s.constants.config[idx], ios, hstep)
+    ==> (forall io :: io in s.t_environment.nextStep.ios && io.LIoOpReceive? ==>
+      // this means that max(replica.ts, msg.ts) <= msg.ts + MaxQueueTime
+      TimeLe(s.t_nodes[idx].ts, io.r.msg.ts + MaxQ)
+    )
+}
+
+predicate ackPacketInv(con:Constants, pkt:TimestampedPbPacket)
+  requires |con.config| > 0
+  requires pkt.msg.v.Ack?
+{
+    TimeLe(pkt.msg.ts, AckPacketT())
+      && pkt.dst == con.config[0]
+}
+
+predicate Inv_AckPacket(ps:TimestampedPbState)
+  requires Consistency(ps)
+{
+  forall pkt :: pkt in ps.t_environment.sentPackets ==> pkt.msg.v.Ack? ==>
+    ackPacketInv(ps.constants, pkt)
+}
+
+lemma lemma_Inv_AckPacket()
+  ensures invImpliesInv(andInv(QAssumption, Inv_RequestPacket), Inv_AckPacket)
+{
+  forall ps, con |
+    TimestampedPbInit(con, ps) && Consistency(ps)
+    && QAssumption(ps) && Inv_RequestPacket(ps)
+    ensures Inv_AckPacket(ps)
+  {}
+
+  forall ps, ps' |
+    TimestampedPbNext(ps, ps') && Consistency(ps) && Consistency(ps') && Inv_AckPacket(ps)
+    && (QAssumption(ps) && Inv_RequestPacket(ps)) && (QAssumption(ps') && Inv_RequestPacket(ps'))
+    ensures Inv_AckPacket(ps')
+  {
+    forall pkt |
+      pkt in ps'.t_environment.sentPackets && pkt.msg.v.Ack?
+      ensures ackPacketInv(ps.constants, pkt)
+    {
+      if pkt in ps.t_environment.sentPackets {
+        assert ackPacketInv(ps.constants, pkt);
+      } else {
+        var i, ios2 :| TimestampedPbNextOneReplica(ps, ps', i, ios2);
+        var ios := ps.t_environment.nextStep.ios;
+        // assert ios[0].r.msg
+        assert ios[0].LIoOpReceive?;
+        lemma_receiveThenSendQ(ps.t_nodes[i].ts, ps'.t_nodes[i].ts,
+            ios[0].r.msg.ts, BackupProcessT, ios[1].s.msg.ts);
+        assert ackPacketInv(ps.constants, pkt);
+      }
+    }
+  }
+}
+
+////////////////////////////////////////////////////////////////////////////////
+
+predicate replyPacketInv(con:Constants, pkt:TimestampedPbPacket)
+  requires |con.config| > 0
+  requires pkt.msg.v.ClientReply?
+{
+    TimeLe(pkt.msg.ts, ReplyPacketT())
+      && pkt.src == con.config[0]
+}
+
+predicate Inv_ReplyPacket(ps:TimestampedPbState)
+  requires Consistency(ps)
+{
+  forall pkt :: pkt in ps.t_environment.sentPackets ==> pkt.msg.v.ClientReply? ==>
+    replyPacketInv(ps.constants, pkt)
+}
+
+lemma lemma_Inv_ReplyPacket()
+  ensures invImpliesInv(andInv(QAssumption, Inv_AckPacket), Inv_ReplyPacket)
+{
+  forall ps, con |
+    TimestampedPbInit(con, ps) && Consistency(ps)
+    && QAssumption(ps) && Inv_AckPacket(ps)
+    ensures Inv_ReplyPacket(ps)
+  {}
+
+  forall ps, ps' |
+    TimestampedPbNext(ps, ps') && Consistency(ps) && Consistency(ps') && Inv_ReplyPacket(ps)
+    && (QAssumption(ps) && Inv_AckPacket(ps)) && (QAssumption(ps') && Inv_AckPacket(ps'))
+    ensures Inv_ReplyPacket(ps')
+  {
+    forall pkt |
+      pkt in ps'.t_environment.sentPackets && pkt.msg.v.ClientReply?
+      ensures replyPacketInv(ps.constants, pkt)
+    {
+      if pkt in ps.t_environment.sentPackets {
+        assert replyPacketInv(ps.constants, pkt);
+      } else {
+        var i, ios2 :| TimestampedPbNextOneReplica(ps, ps', i, ios2);
+        var ios := ps.t_environment.nextStep.ios;
+        // assert ios[0].r.msg
+        assert ios[0].LIoOpReceive?;
+
+        assert i == 0;
+        assert ps.t_nodes[0].v.nextStep == 1;
+
+        lemma_receiveThenSendQ(ps.t_nodes[i].ts, ps'.t_nodes[i].ts,
+            ios[0].r.msg.ts, PrimaryAckT, ios[1].s.msg.ts);
+        assert replyPacketInv(ps.constants, pkt);
+      }
+    }
+  }
+}
+
+
+////////////////////////////////////////////////////////////////////////////////
+
+predicate performanceGuarantee(ps:TimestampedPbState)
+{
+  forall pkt :: pkt in ps.t_environment.sentPackets ==> pkt.msg.v.ClientReply? ==> TimeLe(pkt.msg.ts, ReplyPacketT())
+}
+
+predicate Inv(ps:TimestampedPbState)
+{
+  Consistency(ps)
+  && Inv_RequestPacket(ps)
+}
+
+lemma topLevel()
+{
+
+}
+
+lemma Init_Inv(con:Constants, ps:TimestampedPbState)
+  requires TimestampedPbInit(con, ps)
+  ensures Inv(ps)
+{
+}
+
+predicate invTrue(inv:InvType)
+{
+  forall b ::
+  && (forall ps :: Consistency(ps) ==> inv.requires(ps))
+  && (forall ps, con :: TimestampedPbInit(con, ps) ==> Consistency(ps) ==> inv(ps))
+  && (forall ps, ps' :: TimestampedPbNext(ps, ps') ==>
+      Consistency(ps) ==> inv(ps) ==> Consistency(ps') ==> inv(ps'))
+}
+
+// is(A) && (A -> B) ==>
+// is(A && B)
+
+lemma Next_Inv (ps:TimestampedPbState, ps':TimestampedPbState)
+  requires Inv(ps)
+  requires TimestampedPbNext(ps, ps')
+  ensures Inv(ps')
+{
+  lemma_Inv_Primary();
+  // isInv(Inv_Primary)
+  lemma_Inv_RequestPacket();
+  // invImpliesInv(Inv_Primary, Inv_RequestPacket)
+  lemma_Inv_AckPacket();
+  // invImpliesInv(andInv(QAssumption, Inv_RequestPacket), Inv_AckPacket)
+  lemma_Inv_ReplyPacket();
+  // invImpliesInv(andInv(QAssumption, Inv_AckPacket), Inv_ReplyPacket)
+
+}
+
+}
