ironfleet/src/Dafny/Distributed/Protocol/Pb/PerformanceProof/TimeBounds.i.dfy
@@ -1,0 +1,31 @@
+// Must be verified with /arith:0
+include "Definitions.i.dfy"
+
+module TimeBounds_i {
+import opened Definitions_i
+
+function RequestPacketT() : Timestamp
+{
+  TimeZero() + PrimaryReqT + D
+}
+
+function AckPacketT() : Timestamp
+{
+  RequestPacketT() + MaxQ + BackupProcessT + D
+}
+
+function ReplyPacketT() : Timestamp
+{
+  AckPacketT() + MaxQ + PrimaryAckT + D
+}
+
+lemma lemma_receiveThenSendQ(nodeTs:Timestamp, nodeTs':Timestamp, inMsgTs:Timestamp, X:Timestamp, outMsgTs:Timestamp)
+  requires TimeLe(nodeTs, inMsgTs + MaxQ)
+  requires TimeLe(nodeTs', TimeMax(nodeTs, inMsgTs) + X)
+  requires TimeLe(outMsgTs, nodeTs' + D)
+
+  ensures  TimeLe(outMsgTs, inMsgTs + MaxQ + X + D)
+{
+}
+
+}
